theories/lang/cpp/parser.v
@@ -4,27 +4,20 @@
  * SPDX-License-Identifier:AGPL-3.0-or-later
  *)
 Require Export
-        Coq.Strings.Ascii
-        Coq.Strings.String
         Coq.Lists.List
         Coq.ZArith.BinInt.
 
 Require Import stdpp.gmap.
-Require Import stdpp.stringmap.
 Require Export bedrock.lang.cpp.ast.
 
 Definition Nanon (ty : globname) : globname :=
-  String "#"%char ty.
+  ("#" ++ ty)%bs.
 
 Definition Talias (underlying : type) (name : globname) : type :=
   underlying.
 
 Definition NStop : list ident := nil.
 
-Bind Scope string_scope with globname.
-Bind Scope string_scope with obj_name.
-Bind Scope string_scope with ident.
-Bind Scope string_scope with localname.
 Bind Scope Z_scope with Z.
 
 Declare Custom Entry cppglobal.
@@ -38,44 +31,44 @@ Notation "` e `" := e (e custom cppglobal at level 200, at level 0) : cppfield_s
 (** this is the compatibility layer, cpp2v generates these definitions
  *)
 (* HACK to get around the fact that [gmap_empty] is opaque. *)
-Local Definition empty_symbols : stringmap ObjValue :=
+Local Definition empty_symbols : symbol_table :=
   Eval vm_compute in gmap_empty.
-Local Definition empty_globals : stringmap GlobDecl :=
+Local Definition empty_globals : type_table :=
   Eval vm_compute in gmap_empty.
-Local Instance gmap_empty_trans {T} : Empty (stringmap T) :=
-  ltac:(let x := eval vm_compute in (∅ : stringmap T) in exact x).
+Local Instance symbol_table_empty_trans : Empty symbol_table := empty_symbols.
+Local Instance type_table_empty_trans : Empty type_table := empty_globals.
 
 Definition Dvar (name : obj_name) (t : type) (init : option Expr) : compilation_unit :=
   {| symbols := {[ name := Ovar t init ]}
-   ; globals := empty_globals |}.
+   ; globals := ∅ |}.
 
 Definition Dfunction    (name : obj_name) (f : Func) : compilation_unit :=
   {| symbols := {[ name := Ofunction f ]}
-   ; globals := empty_globals |}.
+   ; globals := ∅ |}.
 Definition Dmethod    (name : obj_name) (f : Method) : compilation_unit :=
   {| symbols := {[ name := Omethod f ]}
-   ; globals := empty_globals |}.
+   ; globals := ∅ |}.
 Definition Dconstructor    (name : obj_name) (f : Ctor) : compilation_unit :=
   {| symbols := {[ name := Oconstructor f ]}
-   ; globals := empty_globals |}.
+   ; globals := ∅ |}.
 Definition Ddestructor    (name : obj_name) (f : Dtor) : compilation_unit :=
   {| symbols := {[ name := Odestructor f ]}
-   ; globals := empty_globals |}.
+   ; globals := ∅ |}.
 Definition Dunion (name : globname) (o : option Union) : compilation_unit :=
-  {| symbols := empty_symbols
+  {| symbols := ∅
    ; globals := {[ name := match o with
                            | None => Gtype
                            | Some u => Gunion u
                            end ]} |}.
 Definition Dstruct (name : globname) (o : option Struct) : compilation_unit :=
-  {| symbols := empty_symbols
+  {| symbols := ∅
    ; globals := {[ name := match o with
                            | None => Gtype
                            | Some u => Gstruct u
                            end ]} |}.
 
 Definition Denum (name : globname) (t : option type) (branches : list (ident * BinNums.Z)) : compilation_unit :=
-  {| symbols := empty_symbols
+  {| symbols := ∅
    ; globals :=
        let enum_ty := Tnamed name in
        let raw_ty :=
@@ -86,22 +79,22 @@ Definition Denum (name : globname) (t : option type) (branches : list (ident * B
        in
        match t with
        | Some t => {[ name := Genum t (List.map fst branches) ]}
-       | None => empty_globals
+       | None => ∅
        end ∪
        list_to_map (List.map (fun '(nm, oe) => (nm, Gconstant enum_ty (Some (Eint oe raw_ty)))) branches) |}.
   (* ^ enumerations (the initializers need to be constant expressions) *)
 
 Definition Dconstant    (name : globname) (t : type) (e : Expr) : compilation_unit :=
-  {| symbols := empty_symbols
+  {| symbols := ∅
    ; globals := {[ name := Gconstant t (Some e) ]} |}.
 Definition Dconstant_undef  (name : globname) (t : type) : compilation_unit :=
-  {| symbols := empty_symbols
+  {| symbols := ∅
    ; globals := {[ name := Gconstant t None ]} |}.
 Definition Dtypedef     (name : globname) (t : type) : compilation_unit :=
-  {| symbols := empty_symbols
+  {| symbols := ∅
    ; globals := {[ name := Gtypedef t ]} |}.
 Definition Dtype (name : globname) : compilation_unit :=
-  {| symbols := empty_symbols
+  {| symbols := ∅
    ; globals := {[ name := Gtype ]}|}.
 
 
@@ -118,7 +111,7 @@ destruct s.
 exists pmap_car. apply Is_true_canon. assumption.
 Defined.
 
-Definition stringmap_canon {K} (s : stringmap K) : stringmap K.
+Definition stringmap_canon {K} (s : gmap bs K) : gmap bs K.
   destruct s.
   refine (
       let t := bool_decide
@@ -143,7 +136,7 @@ Definition compilation_union_canon (c : compilation_unit) : compilation_unit :=
 
 Fixpoint decls' (ls : list compilation_unit) : compilation_unit :=
   match ls with
-  | nil => {| symbols := empty_symbols ; globals := empty_globals |}
+  | nil => {| symbols := ∅ ; globals := ∅ |}
   | m :: ms =>
     let res := decls' ms in
     {| symbols := m.(symbols) ∪ res.(symbols)
@@ -166,9 +159,10 @@ Declare Reduction reduce_compilation_unit :=
         insert map_insert
         partial_alter gmap.gmap_partial_alter pmap.Ppartial_alter pmap.Ppartial_alter_raw
         countable.encode
-        option_union_with string_countable
-        string_to_pos digits_to_pos ascii_to_digits Papp
-        gmap_empty_trans empty pmap.Psingleton_raw flip mbind compose option_bind
+        option_union_with byte_countable
+        Bytestring.print Bytestring.parse Bytestring.t_dec bytestring_countable bytestring.append
+        Papp
+        empty pmap.Psingleton_raw flip mbind compose option_bind
         pmap.PNode'
         List.map fst snd
         list_to_map
@@ -176,8 +170,19 @@ Declare Reduction reduce_compilation_unit :=
         names.localname_eq
         names.ident_eq
         names.obj_name_eq
-        string_rec string_rect string_eq_dec decide_rel ascii_rec ascii_rect
-        ascii_eq_dec ascii_dec negb
+        string_rec string_rect decide_rel
+        negb
         foldr Ascii.shift
 
-        Is_true_canon bool_decide map_Forall_dec map_to_list decide curry pmap.Pto_list list.Forall_dec list.Forall_Exists_dec countable.decode zero string_of_pos string_of_digits shift digits_of_pos ascii_of_digits pmap.Pto_list_raw from_option List.app curry_dec Preverse decide_rel option_eq_dec fmap option_fmap option_map numbers.positive_eq_dec Pos.eq_dec positive_rec positive_rect Preverse_go sumbool_rect sumbool_rec ].
+        symbol_table_empty_trans type_table_empty_trans parser.empty_symbols parser.empty_globals
+
+        list_countable
+        option_ret option_bind mret mbind mapM list_rect list_fmap list_eq_dec
+        positives_flatten N_countable positives_unflatten positives_flatten_go Byte.to_N Byte.of_N
+
+positives_unflatten_go Pdup Pos.succ
+Pos.pred_N Pos.pred_double
+
+        Is_true_canon bool_decide map_Forall_dec map_to_list decide curry pmap.Pto_list list.Forall_dec list.Forall_Exists_dec countable.decode shift pmap.Pto_list_raw from_option List.app curry_dec Preverse decide_rel option_eq_dec fmap option_fmap option_map numbers.positive_eq_dec Pos.eq_dec positive_rec positive_rect Preverse_go sumbool_rect sumbool_rec ].
+
+Export Bytestring.
