theories/bytestring.v
@@ -1,0 +1,162 @@
+(*
+ * Copyright (C) BedRock Systems Inc. 2019 Gregory Malecha
+ *
+ * SPDX-License-Identifier:AGPL-3.0-or-later
+ *)
+Require Import Coq.Strings.String.
+Require Import stdpp.countable.
+
+Set Primitive Projections.
+
+(** bytes *)
+Instance byte_dec : EqDecision Byte.byte := Byte.byte_eq_dec.
+
+Instance byte_countable : Countable Byte.byte.
+refine {| encode x := encode (Byte.to_N x)
+        ; decode x := Byte.of_N (Pos.pred_N x) |}.
+abstract (intros; destruct x; reflexivity).
+Defined.
+
+
+Definition byte_parse (b : Byte.byte) : Byte.byte := b.
+Definition byte_print (b : Byte.byte) : Byte.byte := b.
+
+Delimit Scope byte_scope with byte.
+String Notation Byte.byte byte_parse byte_print : byte_scope.
+
+Bind Scope byte_scope with Byte.byte.
+
+(** bytestrings *)
+Module Bytestring.
+  Inductive t : Set :=
+  | EmptyString
+  | String (_ : Byte.byte) (_ : t).
+
+  Fixpoint print (b : t) : list Byte.byte :=
+    match b with
+    | EmptyString => nil
+    | String b bs => b :: print bs
+    end.
+
+  Fixpoint parse (b : list Byte.byte) : t :=
+    match b with
+    | nil => EmptyString
+    | b :: bs => String b (parse bs)
+    end.
+
+  Lemma print_parse_inv:
+    ∀ x : Bytestring.t, Bytestring.parse (Bytestring.print x) = x.
+  Proof.
+    induction x; simpl; intros; auto.
+    f_equal; auto.
+  Qed.
+
+  Instance t_dec : EqDecision t.
+  Proof. solve_decision. Defined.
+End Bytestring.
+
+Definition bs := Bytestring.t.
+
+Declare Scope bs_scope.
+Delimit Scope bs_scope with bs.
+Bind Scope bs_scope with bs.
+
+String Notation Bytestring.t Bytestring.parse Bytestring.print : bs_scope.
+
+Instance bytestring_countable : Countable bs.
+refine {| encode x := encode (Bytestring.print x)
+        ; decode x := match decode x with
+                      | None => None
+                      | Some y => Some (Bytestring.parse y)
+                      end |}.
+{ induction x; simpl.
+  - reflexivity.
+  - rewrite decode_encode in *. simpl in *.
+    injection IHx; intro; subst.
+    rewrite Bytestring.print_parse_inv. reflexivity. }
+Defined.
+
+Import Bytestring.
+
+Fixpoint append (x y : bs) : bs :=
+  match x with
+  | Bytestring.EmptyString => y
+  | Bytestring.String x xs => Bytestring.String x (append xs y)
+  end.
+
+Notation "x ++ y" := (append x y) : bs_scope.
+
+Fixpoint to_string (b : bs) : string :=
+  match b with
+  | EmptyString => String.EmptyString
+  | String x xs => String.String (Ascii.ascii_of_byte x) (to_string xs)
+  end.
+
+Fixpoint of_string (b : string) : bs :=
+  match b with
+  | String.EmptyString => ""
+  | String.String x xs => String (Ascii.byte_of_ascii x) (of_string xs)
+  end%bs.
+
+Fixpoint rev (acc s : bs) : bs :=
+  match s with
+  | EmptyString => acc
+  | String s ss => rev (String s acc) ss
+  end.
+
+Fixpoint prefix (s1 s2 : bs) {struct s1} : bool :=
+  match s1 with
+  | EmptyString => true
+  | String x xs =>
+    match s2 with
+    | EmptyString => false
+    | String y ys =>
+      if decide (x = y) then prefix xs ys
+      else false
+    end
+  end%bs.
+
+Fixpoint index (n : nat) (s1 s2 : bs) {struct s2} : option nat :=
+  match s2 with
+  | EmptyString =>
+      match n with
+      | 0 => match s1 with
+             | "" => Some 0
+             | String _ _ => None
+             end
+      | S _ => None
+      end
+  | String _ s2' =>
+      match n with
+      | 0 =>
+          if prefix s1 s2
+          then Some 0
+          else match index 0 s1 s2' with
+               | Some n0 => Some (S n0)
+               | None => None
+               end
+      | S n' => match index n' s1 s2' with
+                | Some n0 => Some (S n0)
+                | None => None
+                end
+      end
+  end%bs.
+
+Fixpoint length (l : bs) : nat :=
+  match l with
+  | EmptyString => 0
+  | String _ l => S (length l)
+  end.
+
+Local Fixpoint contains (start: nat) (keys: list bs) (fullname: bs) :bool :=
+  match keys with
+  | kh::ktl =>
+    match index start kh fullname with
+    | Some n => contains (n + length kh) ktl fullname
+    | None => false
+    end
+  | [] => true
+  end.
+
+Definition eqb (a b : bs) : bool :=
+  if decide (a = b) then true else false.
