theories/lang/cpp/logic/heap_pred.v
@@ -15,8 +15,6 @@ From bedrock.lang.cpp Require Import
      semantics logic.pred logic.path_pred ast logic.wp.
 Require Import bedrock.lang.cpp.logic.spec.
 
-Local Open Scope string_scope.
-
 Set Default Proof Using "Type".
 
 Lemma monPred_at_persistent_inv {V bi} (P : monPred V bi) :
